theories/Imp.v
@@ -1,397 +1,667 @@
-From Coq Require Import Strings.String Bool.
-Require Import StateMap.
+From Stdlib Require Import Arith ZArith Psatz Bool String List Program.Equality.
+From IncLogic Require Import Sequences.
 
 Local Open Scope string_scope.
 Local Open Scope Z_scope.
 Local Open Scope list_scope.
 
+(** * 1.  The IMP language *)
+
+(** ** 1.1 Arithmetic expressions *)
+
 Definition ident := string.
 
+(** The abstract syntax: an arithmetic expression is either... *)
+
 Inductive aexp : Type :=
-  | ANum (n : nat)
-  | AId (x : ident)
-  | APlus (a1 a2 : aexp)
-  | AMinus (a1 a2 : aexp)
-  | AMult (a1 a2 : aexp)
-.
+  | CONST (n: Z)                       (**r a constant, or *)
+  | VAR (x: ident)                     (**r a variable, or *)
+  | PLUS (a1: aexp) (a2: aexp)         (**r a sum of two expressions, or *)
+  | MINUS (a1: aexp) (a2: aexp).       (**r a difference of two expressions *)
 
-Inductive bexp : Type :=
-  | BTrue
-  | BFalse
-  | BEq (a1 a2 : aexp)
-  | BNot (b : bexp)
-  | BLessEqual (a1 a2 : aexp)
-  | BAnd (a1 a2 : bexp)
-.
+Definition store : Type := ident -> Z.
 
-Inductive com : Type :=
-  | Skip
-  | Asign: string -> aexp -> com
-  | Seq : com -> com -> com
-  | Assume : bexp -> com
-  | Error: com
-  | Star: com -> com                   (* Kleene iteration *)
-  | Choice: com -> com -> com          (* Kleene algebra union *)
-  | CLocal: string -> com -> com
-  | Nondet: string -> com.             (* Nondet Assignment *)
-
-Coercion AId : ident >-> aexp.
-
-Coercion ANum : nat >-> aexp.
-
-Declare Custom Entry com.
-
-Declare Scope com_scope.
-
-Notation "<{ e }>" := e (at level 0, e custom com at level 99) : com_scope.
-Notation "( x )" := x (in custom com, x at level 99) : com_scope.
-Notation "x" := x (in custom com at level 0, x constr at level 0) : com_scope.
-Notation "f x .. y" := (.. (f x) .. y)
-                  (in custom com at level 0, only parsing,
-                  f constr at level 0, x constr at level 9,
-                  y constr at level 9) : com_scope.
-Notation "x + y" := (APlus x y) (in custom com at level 70, left associativity).
-Notation "x - y" := (AMinus x y) (in custom com at level 70, left associativity).
-Notation "x * y" := (AMult x y) (in custom com at level 50, left associativity).
-Notation "'true'" := true (at level 1).
-Notation "'true'" := BTrue (in custom com at level 0).
-Notation "'false'" := false (at level 1).
-Notation "'false'" := BFalse (in custom com at level 0).
-Notation "x = y" := (BEq x y) (in custom com at level 70, no associativity).
-Notation "'~' b" := (BNot b) (in custom com at level 75, right associativity).
-Notation "a //\\ b" := (BAnd a b) (in custom com at level 60, right associativity).
-Notation "a <= b" := (BLessEqual a b) (in custom com at level 60).
-Notation "'~' b" := (BNot b) (in custom com at level 75, right associativity).
-Open Scope com_scope.
-
-(* Eval compute in  InA_cons_hd M.E ("Y"%string :: "X"%string :: nil). *)
-
-(* witch to aevalR *)
-Fixpoint aeval (st : state) (a : aexp) : option nat :=
+Fixpoint aeval (a: aexp) (s: store) : Z :=
   match a with
-  | ANum n => Some n
-  | AId x => StateMap.get st x
-  | <{a1 + a2}> => 
-      match (aeval st a1), (aeval st a2) with
-      | Some va1, Some va2 => Some (va1 + va2)
-      | _, _ => None
-      end
-  | <{a1 - a2}> => match (aeval st a1), (aeval st a2) with
-      | Some va1, Some va2 => Some (va1 - va2)
-      | _, _ => None
-      end
-  | <{a1 * a2}> => match (aeval st a1), (aeval st a2) with
-      | Some va1, Some va2 => Some (va1 * va2)
-      | _, _ => None
-      end
+  | CONST n => n
+  | VAR x => s x
+  | PLUS a1 a2 => aeval a1 s + aeval a2 s
+  | MINUS a1 a2 => aeval a1 s - aeval a2 s
   end.
 
-Definition NOTEQUAL (a1 a2: aexp) : bexp := <{~ (a1 = a2)}>.
+Eval compute in (aeval (PLUS (VAR "x") (MINUS (VAR "x") (CONST 1)))  (fun x => 2)).
 
-Definition GREATEREQUAL (a1 a2: aexp) : bexp := <{ a2 <= a1 }>.
+Eval cbn in (aeval (PLUS (VAR "x") (MINUS (CONST 10) (CONST 1)))) (fun x => 2).
 
-Definition GREATER (a1 a2: aexp) : bexp := <{~ (a1 <= a2)}>.
+(** Result: [ = fun s : store => s "x" + 9 ]. *)
 
-Definition LESS (a1 a2: aexp) : bexp := GREATER a2 a1.
+(** We can prove mathematical properties of a given expression. *)
 
-Definition OR (b1 b2: bexp) : bexp := <{~ ((~ b1) //\\ (~ b2))}>.
-
-Notation "a \\// b" := (OR a b) (in custom com at level 80, right associativity).
-
-
-Definition equal_option [A B] (eq : A -> B -> bool) (a : option A) (b : option B) : bool
-  := match a with
-     | None => match b with
-               | None => true
-               | _ => false
-               end
-     | Some a => match b with
-                 | Some b => eq a b
-                 | _ => false
-                 end
-     end.
-
-Fixpoint beval (st : state) (b : bexp): bool :=
-  match b with
-  | BTrue => true
-  | BFalse => false
-  | BEq a1 a2 => equal_option (Nat.eqb) (aeval st a1) (aeval st a2)
-  | BLessEqual a1 a2 => equal_option (Nat.leb) (aeval st a1) (aeval st a2)
-  | BAnd b1 b2 => andb (beval st b1) (beval st b2)
-  | BNot b1 => negb (beval st b1)
-  end.
-
-Lemma beval_OR:
-  forall st b1 b2, beval st <{b1 \\// b2}> = beval st b1 || beval st b2.
+Lemma aeval_xplus1:
+  forall s x, aeval (PLUS (VAR x) (CONST 1)) s > aeval (VAR x) s.
 Proof.
-  intros. cbn.
-  rewrite negb_andb.
-  do 2 rewrite negb_involutive.
-  reflexivity.
+  intros. cbn. lia.
 Qed.
 
-(*
-  The value of an expression depends only on the values of its free variables.
+(** Finally, we can prove "meta-properties" that hold for all expressions.
+  For example: the value of an expression depends only on the values of its
+  free variables.
 
   Free variables are defined by this recursive predicate:
 *)
 Fixpoint free_in_aexp (x: ident) (a: aexp) : Prop :=
   match a with
-  | ANum n => False
-  | AId y => y = x
-  | APlus a1 a2 | AMinus a1 a2 | AMult a1 a2 => free_in_aexp x a1 \/ free_in_aexp x a2
+  | CONST n => False
+  | VAR y => y = x
+  | PLUS a1 a2 | MINUS a1 a2 => free_in_aexp x a1 \/ free_in_aexp x a2
   end.
 
 Theorem aeval_free:
   forall s1 s2 a,
-  (forall x, free_in_aexp x a -> get s1 x = get s2 x) ->
-  aeval s1 a  = aeval s2 a .
+  (forall x, free_in_aexp x a -> s1 x = s2 x) ->
+  aeval a s1 = aeval a s2.
 Proof.
-  induction a; cbn; intros Hfree; auto.
-  all: (rewrite IHa1, IHa2; auto).
+  induction a; cbn; intros SAMEFREE.
+- (* Case a = CONST n *)
+  auto.
+- (* Case a = VAR x *)
+  apply SAMEFREE. auto.
+- (* Case a = PLUS a1 a2 *)
+  rewrite IHa1, IHa2; auto.
+- (* Case a = MINUS a1 a2 *)
+  rewrite IHa1, IHa2; auto.
+Qed.
+
+Definition OPP (a: aexp) : aexp := MINUS (CONST 0) a.
+
+Lemma aeval_OPP: forall s a, aeval (OPP a) s = - (aeval a s).
+Proof.
+  intros; cbn. lia.
+Qed.
+
+(** The IMP language has conditional statements (if/then/else) and
+  loops.  They are controlled by expressions that evaluate to Boolean
+  values.  Here is the abstract syntax of Boolean expressions. *)
+
+Inductive bexp : Type :=
+  | TRUE                              (**r always true *)
+  | FALSE                             (**r always false *)
+  | EQUAL (a1: aexp) (a2: aexp)       (**r whether [a1 = a2] *)
+  | LESSEQUAL (a1: aexp) (a2: aexp)   (**r whether [a1 <= a2] *)
+  | EVEN (a1: aexp)                   (**r whether [a1] evaluates to an even integer *)
+  | NOT (b1: bexp)                    (**r Boolean negation *)
+  | AND (b1: bexp) (b2: bexp).        (**r Boolean conjunction *)
+
+(** Just like arithmetic expressions evaluate to integers,
+  Boolean expressions evaluate to Boolean values [true] or [false]. *)
+
+Fixpoint beval (b: bexp) (s: store) : bool :=
+  match b with
+  | TRUE => true
+  | FALSE => false
+  | EQUAL a1 a2 => aeval a1 s =? aeval a2 s
+  | LESSEQUAL a1 a2 => aeval a1 s <=? aeval a2 s
+  | EVEN a1 => Z.even (aeval a1 s)
+  | NOT b1 => negb (beval b1 s)
+  | AND b1 b2 => beval b1 s && beval b2 s
+  end.
+
+(** There are many useful derived forms. *)
+
+Definition NOTEQUAL (a1 a2: aexp) : bexp := NOT (EQUAL a1 a2).
+
+Definition GREATEREQUAL (a1 a2: aexp) : bexp := LESSEQUAL a2 a1.
+
+Definition GREATER (a1 a2: aexp) : bexp := NOT (LESSEQUAL a1 a2).
+
+Definition LESS (a1 a2: aexp) : bexp := GREATER a2 a1.
+
+Definition OR (b1 b2: bexp) : bexp := NOT (AND (NOT b1) (NOT b2)).
+
+(** Derived form: evenness test on arithmetic expressions. *)
+Definition ODD (a: aexp) : bexp := NOT (EVEN a).
+
+(** ** 1.2 Commands *)
+Declare Custom Entry com.
+Declare Scope com_scope.
+Delimit Scope com_scope with com.
+Local Open Scope com_scope.
+
+Notation "x + y" := (PLUS x y) (in custom com at level 50, left associativity).
+Notation "x - y" := (MINUS x y) (in custom com at level 50, left associativity).
+
+(**  Commands *)
+
+Inductive com: Type :=
+  | SKIP                         (**r do nothing *)
+  | ERROR                        (**r interrupt the program *)
+  | ASSIGN (x: ident) (a: aexp)  (**r assignment: [v := a] *)
+  | NONDET (x: ident)            (**r non-deterministic assignment to [x] *)
+  | ASSUME (b: bexp)             (**r assume that [b] holds *)
+  | SEQ (c1: com) (c2: com)      (**r sequence: [c1; c2] *)
+  | CHOICE (c1: com) (c2: com)   (**r non-deterministic choice: [c1 + c2] *)
+  | CSTAR (c1: com).             (**r non-deterministic iteration: [c1★] *)
+
+(** We can write [c1 ;; c2] instead of [SEQ c1 c2], it is easier on the eyes. *)
+
+Infix ";;" := SEQ (at level 80, right associativity).
+
+Notation "c1 '⊕' c2" := (CHOICE c1 c2)
+                         (in custom com at level 85, right associativity).
+
+Notation "c '★'" := (CSTAR c)
+                         (in custom com at level 90, right associativity).
+
+Notation "c '★'" := (CSTAR c)
+                         (at level 90, right associativity) : com_scope.
+
+(** We can now define the syntax of while-loops in terms of the core IMP commands. *)
+Notation "'WHILE' b 'DO' c 'END'" :=
+  (((ASSUME b ;; c) ★) ;; ASSUME (NOT b))
+    (at level 95, right associativity) : com_scope.
+
+(** Similarly, we can define conditional statements.
+
+    Note: Coq does not handle an “optional ELSE” well when both notations
+    start with exactly the same prefix [IF ... THEN ...].
+
+    To keep the convenient no-ELSE syntax, we reserve [IF ... THEN ... END]
+    for the no-ELSE form, and introduce a separate keyword [IFELSE] for the
+    form with [ELSE]. *)
+Notation "'IF' b 'THEN' c1 'ELSE' c2 'END'" :=
+  (CHOICE
+     (ASSUME b ;; c1)
+     (ASSUME (NOT b) ;; c2))
+    (at level 89, right associativity,
+     b at level 99,
+     c1 at level 89,
+     c2 at level 89) : com_scope.
+
+Notation "'IF' b 'THEN' c1 'END'" :=
+  (IF b THEN c1 ELSE SKIP END)
+  (at level 90, right associativity,
+   b at level 99,
+   c1 at level 89,
+   only parsing) : com_scope.
+
+Notation "'ASSERT' b" :=
+  (CHOICE
+     (ASSUME b)
+     (ASSUME (NOT b) ;; ERROR))
+    (at level 100, right associativity) : com_scope.
+
+(** Here is an example arithmetic expression: *)
+
+(** Here is an example IMP program that computes the Euclidean division
+    of two natural numbers [a] and [b], storing the quotient in variable
+    ["q"] and the remainder in variable ["r"].  We assume that [b > 0]. *)
+
+Definition Euclidean_division: com :=
+  ASSIGN "r" (VAR "a") ;;
+  ASSIGN "q" (CONST 0) ;;
+  WHILE (LESSEQUAL (VAR "b") (VAR "r")) DO
+    (ASSIGN "r" (MINUS (VAR "r") (VAR "b")) ;;
+     ASSIGN "q" (PLUS (VAR "q") (CONST 1)))
+  END.
+
+(** Example in section 3.1 *)
+Definition Under_approximating_ex: com :=
+  IF (EVEN (VAR "x")) THEN
+    IF (ODD (VAR "y")) THEN
+      ASSIGN "z" (CONST 42)
+    ELSE
+      SKIP
+    END
+  END.
+
+(** ** 1.3 Small-step operational semantics *)
+
+(** A useful operation over stores:
+    [update x v s] is the store that maps [x] to [v] and is equal to [s] for
+    all variables other than [x]. *)
+
+Definition update (x: ident) (v: Z) (s: store) : store :=
+  fun y => if string_dec x y then v else s y.
+
+Lemma update_same: forall x v s, (update x v s) x = v.
+Proof.
+  unfold update; intros. destruct (string_dec x x); congruence.
+Qed.
+
+Lemma update_other: forall x v s y, x <> y -> (update x v s) y = s y.
+Proof.
+  unfold update; intros. destruct (string_dec x y); congruence.
+Qed.
+
+(** The result type indicates the end value of a program, either a state or an error *)
+Inductive result : Type :=
+| RNormal : store -> result
+| RError : result.
+
+(** The relation [ red (c, s) (c', s') ] defines a basic reduction,
+    that is, the first computation step when executing command [c]
+    in initial memory state [s].
+    [s'] is the memory state "after" this computation step.
+    [c'] is a command that represent all the computations that remain
+    to be performed later.
+
+    The reduction relation is presented as a Coq inductive predicate,
+    with one case (one "constructor") for each reduction rule.
+*)
+
+Inductive red: com * store -> com * store -> Prop :=
+  | red_assign: forall x a s,
+      red (ASSIGN x a, s) (SKIP, update x (aeval a s) s)
+  | red_nondet: forall x s n,
+    red (NONDET x, s) (SKIP, update x n s)
+  | red_assume_true: forall b s,
+    (* beval b s = true -> *)
+    red (ASSUME b, s) (SKIP, s)
+  (* | red_assume_false: forall b s,
+    beval b s = false ->
+    red (ASSUME b, s) (ERROR, s) *)
+  | red_seq_done: forall c s,
+      red (SEQ SKIP c, s) (c, s)
+  | red_seq_error: forall c s,
+    red (SEQ ERROR c, s) (ERROR, s)
+  | red_seq_step: forall c1 c s1 c2 s2,
+      red (c1, s1) (c2, s2) ->
+      red (SEQ c1 c, s1) (SEQ c2 c, s2)
+  | red_choice_left: forall c1 c2 s,
+      red (CHOICE c1 c2, s) (c1, s)
+  | red_choice_right: forall c1 c2 s,
+      red (CHOICE c1 c2, s) (c2, s)
+  | red_cstar_done: forall c s,
+      red (CSTAR c, s) (SKIP, s)
+  | red_cstar_step: forall c s,
+      red (CSTAR c, s) (SEQ c (CSTAR c), s).
+
+(** Final configurations for the small-step semantics, corresponding to [result]. *)
+Inductive final : com * store -> result -> Prop :=
+  | final_skip : forall s,
+    final (SKIP, s) (RNormal s)
+  | final_error : forall s,
+    final (ERROR, s) RError.
+
+  (** Termination for the small-step semantics that returns a [result]. *)
+  Definition terminates_result (s: store) (c: com) (r: result) : Prop :=
+    exists cs, star red (c, s) cs /\ final cs r.
+
+(** This IMP language is not deterministic due to the nondeterministic choice (+) operator *)
+Lemma red_nondeterm :
+  exists cs cs1 cs2,
+    red cs cs1 /\ red cs cs2 /\ cs1 <> cs2.
+Proof.
+  exists (CHOICE SKIP (ASSIGN "x" (CONST 1)), fun x => 0).
+  exists (SKIP, fun x => 0).
+  exists (ASSIGN "x" (CONST 1), fun x => 0).
+  split.
+  - apply red_choice_left.
+  - split.
+    + apply red_choice_right.
+    + intro. discriminate H.
+Qed.
+
+(** We define the semantics of a command by chaining successive reductions.
+    The command [c] in initial state [s] terminates with final state [s']
+    if we can go from [(c, s)] to [(skip, s')] in a finite number of reductions.
+*)
+
+Definition terminates (s: store) (c: com) (s': store) : Prop :=
+  star red (c, s) (SKIP, s').
+
+(** The [star] operator is defined in library [Sequences].
+    [star R] is the reflexive transitive closure of relation [R].
+    On paper it is often written [R*].
+    The [star red] relation therefore represents zero, one or several
+    reduction steps. *)
+
+(** Likewise, command [c] diverges (fails to terminate) in initial state [s]
+    if there exists an infinite sequence of reductions starting with [(c, s)].
+    The [infseq] relation operator is defined in library [Sequences].
+*)
+
+Definition diverges (s: store) (c: com) : Prop :=
+  infseq red (c, s).
+
+(** Generally speaking, a third kind of executions is possible:
+    "going wrong" after a finite number of reductions.
+   A configuration [(c', s')] "goes wrong" if it cannot reduce and is
+   not a final configuration, that is, [c' <> SKIP] and [c' <> ERROR]. *)
+
+Definition goes_wrong (s: store) (c: com) : Prop :=
+  exists c', exists s',
+  star red (c, s) (c', s') /\ irred red (c', s') /\ c' <> SKIP /\ c' <> ERROR.
+
+(** A command other than [SKIP] can always reduce. *)
+Lemma red_progress:
+  forall c s,
+    c = SKIP \/ c = ERROR \/ exists c', exists s', red (c, s) (c', s').
+Proof.
+  induction c; intros.
+  - left. reflexivity.
+  - right. left. reflexivity.
+  - right. right. exists SKIP. exists (update x (aeval a s) s). apply red_assign.
+  - right. right. exists SKIP. exists (update x 0 s). apply red_nondet.
+  - right. right.  exists SKIP. exists s. apply red_assume_true.
+    (* destruct (beval b s) eqn:HB.
+     + exists SKIP. exists s. apply red_assume_true. (* exact HB. *)
+    + exists ERROR. exists s. apply red_assume_false. exact HB. *)
+  - (* SEQ *)
+    specialize (IHc1 s) as [Hskip | [Herror | (c' & s' & STEP)]].
+    + subst. right. right. exists c2. exists s. apply red_seq_done.
+    + subst. right. right. exists ERROR. exists s. apply red_seq_error.
+    + right. right. exists (SEQ c' c2). exists s'. apply red_seq_step. exact STEP.
+  - right. right. exists c1. exists s. apply red_choice_left.
+  - right. right. exists SKIP. exists s. apply red_cstar_done.
+Qed.
+
+Lemma not_goes_wrong:
+  forall c s, ~(goes_wrong s c).
+Proof.
+  intros c s (c' & s' & STAR & IRRED & NOTSKIP & NOTERROR).
+  (* If [(c',s')] is reachable and [c'] is neither final form, then it must be
+     able to take a reduction step (by [red_progress]), contradicting [irred]. *)
+  destruct (red_progress c' s') as [EQSKIP | [EQERROR | (c'' & s'' & STEP)]].
+  - contradiction.
+  - contradiction.
+  - unfold irred in IRRED. specialize (IRRED (c'', s'') STEP). contradiction.
+Qed.
+
+(* * A technical lemma: a sequence of reductions can take place to the left
+    of a [SEQ] constructor.  This generalizes rule [red_seq_step]. *)
+Lemma red_seq_steps:
+  forall c2 s c s' c',
+  star red (c, s) (c', s') -> star red ((c ;; c2), s) ((c' ;; c2), s').
+Proof.
+  intros. dependent induction H.
+- apply star_refl.
+- destruct b as [c1 st1].
+  apply star_step with (c1;;c2, st1). apply red_seq_step. auto. auto.  
+Qed.
+
+(** Natural semantics *)
+
+Reserved Notation "st0 =[ c ]=> st1"
+  (at level 40, c at level 99, st1 at level 39).
+
+Inductive cexec: store -> com -> result -> Prop :=
+  | cexec_skip: forall s,
+      s =[ SKIP ]=> RNormal s
+  | cexec_error: forall s,
+      s =[ ERROR ]=> RError
+  | cexec_assign: forall s x a,
+    s =[ ASSIGN x a ]=> RNormal (update x (aeval a s) s)
+  | cexec_nondet: forall s x n,
+    s =[ NONDET x ]=> RNormal (update x n s)
+  | cexec_assume: forall s b,
+    (* beval b s = true -> *)
+    s =[ ASSUME b ]=> RNormal s
+  (* | cexec_assume_false: forall s b,
+    beval b s = false ->
+    s =[ ASSUME b ]=> RError *)
+  | cexec_seq: forall c1 c2 s s' s'',
+    s  =[ c1 ]=> RNormal s' ->
+    s' =[ c2 ]=> RNormal s'' ->
+    s  =[ SEQ c1 c2 ]=> RNormal s''
+  | cexec_seq_error: forall c1 c2 s,
+    s  =[ c1 ]=> RError ->
+    s  =[ SEQ c1 c2 ]=> RError
+  | cexec_seq_error_right: forall c1 c2 s s',
+    s  =[ c1 ]=> RNormal s' ->
+    s' =[ c2 ]=> RError ->
+    s  =[ SEQ c1 c2 ]=> RError
+  | cexec_choice_left: forall s c1 c2 r,
+    s =[ c1 ]=> r ->
+    s =[ CHOICE c1 c2 ]=> r
+  | cexec_choice_right: forall s c1 c2 r,
+    s =[ c2 ]=> r ->
+    s =[ CHOICE c1 c2 ]=> r
+  | cexec_cstar_done: forall c s,
+    s =[ CSTAR c ]=> RNormal s
+  | cexec_cstar_step_ok: forall c s s' r,
+    s  =[ c ]=> RNormal s' ->
+    s' =[ CSTAR c ]=> r ->
+    s  =[ CSTAR c ]=> r
+  | cexec_cstar_step_error: forall c s,
+    s  =[ c ]=> RError ->
+    s  =[ CSTAR c ]=> RError
+  where "st0 =[ c ]=> st1" := (cexec st0 c st1).
+
+Notation "s1 =[ c ]=> 'ok' ↑ s2" := (cexec s1 c (RNormal s2))
+  (at level 40, c at level 99, s2 at level 39).
+
+Notation "s1 =[ c ]=> 'err'" := (cexec s1 c RError)
+  (at level 40, c at level 99).
+
+(** We now show an equivalence between evaluations that terminate according
+    to the natural semantics
+        (existence of a derivation of [cexec s c s'])
+    and to the reduction semantics
+        (existence of a reduction sequence from [(c,s)] to [(SKIP, s')].
+
+    We start with the natural semantics => reduction sequence direction,
+    which is proved by an elegant induction on the derivation of [cexec]. *)
+
+Theorem cexec_to_reds:
+  forall s c r, cexec s c r -> terminates_result s c r.
+Proof.
+  induction 1.
+  - (* SKIP *)
+    exists (SKIP, s). split.
+    + apply star_refl.
+    + apply final_skip.
+  - (* ERROR *)
+    exists (ERROR, s). split.
+    + apply star_refl.
+    + apply final_error.
+  - (* ASSIGN *)
+    exists (SKIP, update x (aeval a s) s). split.
+    + apply star_one. apply red_assign.
+    + apply final_skip.
+  - (* NONDET *)
+    exists (SKIP, update x n s). split.
+    + apply star_one. apply red_nondet.
+    + apply final_skip.
+  - (* ASSUME true *)
+    exists (SKIP, s). split.
+     + apply star_one. apply red_assume_true. (*exact H. *)
+    + apply final_skip.
+   (*-  ASSUME false *)
+    (* exists (ERROR, s). split.
+    + apply star_one. apply red_assume_false. exact H.
+    + apply final_error. *)
+  - (* SEQ normal *)
+    destruct IHcexec1 as (cs1 & STAR1 & FINAL1).
+    inversion FINAL1; subst cs1.
+    destruct IHcexec2 as (cs2 & STAR2 & FINAL2).
+    inversion FINAL2; subst cs2.
+    exists (SKIP, s''). split.
+    + eapply star_trans.
+      * apply red_seq_steps with (c2 := c2) in STAR1. exact STAR1.
+      * eapply star_step. apply red_seq_done. subst. exact STAR2.
+    + apply final_skip.
+  - (* SEQ error (left) *)
+    destruct IHcexec as (cs1 & STAR1 & FINAL1).
+    inversion FINAL1; subst cs1.
+    exists (ERROR, s0). split.
+    + eapply star_trans.
+      * apply red_seq_steps with (c2 := c2) in STAR1. exact STAR1.
+      * apply star_one. apply red_seq_error.
+    + apply final_error.
+  - (* SEQ error (right) *)
+    destruct IHcexec1 as (cs1 & STAR1 & FINAL1).
+    inversion FINAL1; subst cs1.
+    destruct IHcexec2 as (cs2 & STAR2 & FINAL2).
+    inversion FINAL2; subst cs2.
+    exists (ERROR, s1). split.
+    + subst.
+      eapply star_trans.
+      * apply red_seq_steps with (c2 := c2) in STAR1. exact STAR1.
+      * eapply star_step.
+        -- apply red_seq_done.
+        -- exact STAR2.
+    + apply final_error.
+  - (* CHOICE left *)
+    destruct IHcexec as (cs & STAR & FINAL').
+    exists cs. split.
+    + eapply star_step. apply red_choice_left. exact STAR.
+    + exact FINAL'.
+  - (* CHOICE right *)
+    destruct IHcexec as (cs & STAR & FINAL').
+    exists cs. split.
+    + eapply star_step. apply red_choice_right. exact STAR.
+    + exact FINAL'.
+  - (* CSTAR done *)
+    exists (SKIP, s). split.
+    + apply star_one. apply red_cstar_done.
+    + apply final_skip.
+  - (* CSTAR step ok *)
+    destruct IHcexec1 as (cs1 & STAR1 & FINAL1).
+    inversion FINAL1; subst cs1.
+    destruct IHcexec2 as (cs2 & STAR2 & FINAL2).
+    exists cs2. split.
+    + eapply star_trans.
+      * apply star_one. apply red_cstar_step.
+      * eapply star_trans.
+        -- apply red_seq_steps with (c2 := CSTAR c) in STAR1. exact STAR1.
+        -- eapply star_step. apply red_seq_done. subst. exact STAR2.
+    + exact FINAL2.
+  - (* CSTAR step error *)
+    destruct IHcexec as (cs1 & STAR1 & FINAL1).
+    inversion FINAL1; subst cs1.
+    exists (ERROR, s0). split.
+    + eapply star_trans.
+      * apply star_one. apply red_cstar_step.
+      * eapply star_trans.
+        -- apply red_seq_steps with (c2 := CSTAR c) in STAR1. exact STAR1.
+        -- apply star_one. apply red_seq_error.
+    + apply final_error.
+Qed.
+
+(* * One full body execution yields at least one [red] step from [c★] to [c★]. *)
+Lemma plus_cstar_iteration:
+  forall c s s',
+    star red (c, s) (SKIP, s') ->
+    plus red (CSTAR c, s) (CSTAR c, s').
+Proof.
+  intros c s s' STARC.
+  eapply plus_left.
+  - apply red_cstar_step.
+  - eapply star_trans.
+    + (* reduce the body on the left of the sequence *)
+      apply red_seq_steps with (c2 := CSTAR c) in STARC.
+      exact STARC.
+    + (* then drop the leading SKIP *)
+      apply star_one. apply red_seq_done.
 Qed.
 
 
-Reserved  Notation "'assume' l " 
-          (in custom com at level 8, l custom com at level 0).
-Reserved Notation "x ; y" (in custom com at level 90, right associativity).
+(** If the body always terminates (and is not [SKIP]), we can repeat it forever,
+    hence there exists an infinite reduction sequence for [c★]. *)
+Lemma diverges_cstar_via_cexec_cstar_step:
+  forall c s,
+    (forall st, exists st', st =[ c ]=> RNormal st') ->
+    diverges s (CSTAR c).
+Proof.
+  intros c s BODY_TERMINATES.
+  unfold diverges.
+  eapply (@infseq_coinduction_principle
+            (com * store)
+            red
+            (fun cs => exists st, cs = (CSTAR c, st))); eauto.
+  intros cs (st0 & EQ). subst cs.
+    destruct (BODY_TERMINATES st0) as (st1 & EXECc).
+    pose proof (cexec_to_reds st0 c (RNormal st1) EXECc) as TERM.
+    destruct TERM as (cs1 & STARc & FINALc).
+    inversion FINALc; subst cs1.
+    exists (CSTAR c, st1). split.
+    + apply plus_cstar_iteration; subst; auto.
+    + exists st1. reflexivity.
+Qed.
 
-Notation "x := y" :=
-         (Asign x y)
-            (in custom com at level 0, x constr at level 0,
-             y at level 85, no associativity) : com_scope.
-Notation "'local' x . C" :=
-        (CLocal x C)
-          (in custom com at level 8, x custom com at level 0) : com_scope.
-Notation "'skip'" :=
-         Skip (in custom com at level 0) : com_scope.
-Notation "x ; y" :=
-         (Seq x y)
-          (in custom com at level 90, right associativity) : com_scope.
-Notation "'assume' l " :=
-        (Assume l)
-          (in custom com at level 8, l custom com at level 0) : com_scope.
-Notation "'nondet' x":=
-        (Nondet x)
-          (in custom com at level 8) : com_scope.
-Notation "'error()'" :=
-          Error (in custom com at level 0) : com_scope.
-Notation "c '⋆'" :=
-        (Star c) (in custom com at level 8) : com_scope.
-Notation "x '⨁' y " :=
-        (Choice x y) (in custom com at level 8) : com_scope.
+(** The other direction, from a reduction sequence to a [cexec]
+    derivation, is more subtle.  Here is the key lemma, showing how a
+    reduction step followed by a [cexec] execution can combine into a
+    [cexec] execution. *)
 
-(* Notations for while, if and assert keywords *)
+Lemma red_append_cexec:
+  forall c1 s1 c2 s2, red (c1, s1) (c2, s2) ->
+  forall s', s2 =[ c2 ]=> s' -> s1 =[ c1 ]=> s'.
+Proof.
+  intros until s2; intros STEP. dependent induction STEP; intros s' EXEC.
+  - (* red_assign *)
+    inversion EXEC; subst. apply cexec_assign.
+  - (* red_nondet *)
+    inversion EXEC; subst. eapply cexec_nondet.
+  - (* red_assume_true *)
+    inversion EXEC; subst. eapply cexec_assume; eauto.
+  (* - red_assume_false *)
+    (* inversion EXEC; subst. eapply cexec_assume_false; eauto. *)
+  - (* red_seq_done  *)
+    destruct s' as [st'|].
+    + apply cexec_seq with s2. apply cexec_skip. exact EXEC.
+    + apply cexec_seq_error_right with s2. apply cexec_skip. exact EXEC.
+  - (* red_seq_error *)
+    inversion EXEC; subst.
+    eapply cexec_seq_error. apply cexec_error.
+  - (* red_seq_step *)
+    inversion EXEC; subst.
+    + (* normal *)
+      eapply cexec_seq.
+      * eapply IHSTEP; eauto.
+      * exact H4.
+    + (* error left *)
+      eapply cexec_seq_error.
+      eapply IHSTEP; eauto.
+    + (* error right *)
+      eapply cexec_seq_error_right.
+      * eapply IHSTEP; eauto.
+      * exact H4.
+  - (* red_choice_left *)
+    apply cexec_choice_left. exact EXEC.
+  - (* red_choice_right *)
+    apply cexec_choice_right. exact EXEC.
+  - (* red_cstar_done *)
+    inversion EXEC; subst. apply cexec_cstar_done.
+  - (* red_cstar_step *)
+    inversion EXEC; subst.
+    + (* normal *)
+      eapply cexec_cstar_step_ok; eauto.
+    + (* error left *)
+      eapply cexec_cstar_step_error; eauto.
+    + (* error right *)
+      eapply cexec_cstar_step_ok; eauto.
+Qed.
 
-Definition While b c := <{ (assume b ; c) ⋆ ; assume ~ b }>.
+(** By induction on the reduction sequence, it follows that a command
+    that terminates according to the small-step semantics executes according
+    to the natural semantics, with the same [result]. *)
+Theorem reds_to_cexec:
+  forall s c r,
+  terminates_result s c r -> s =[ c ]=> r.
+Proof.
+  intros s c r (cs & STAR & FINAL).
+  dependent induction STAR.
+  - inversion FINAL; subst; constructor.
+  - destruct b as [c2 s2].
+    eapply red_append_cexec; eauto.
+Qed.
 
-Notation "'while' b 'do' c" :=
-  (While b c)
-  (in custom com at level 10, b at next level, c at next level) : com_scope.
+Corollary reds_to_cexec_normal:
+  forall s c s',
+    star red (c, s) (SKIP, s') -> s =[ c ]=> RNormal s'.
+Proof.
+  intros s c s' STAR.
+  apply reds_to_cexec.
+  exists (SKIP, s'). split; [exact STAR | constructor].
+Qed.
 
-Definition If b c c' := <{ (assume b ; c) ⨁ ((assume ~ b) ; c') }>.
-
-Notation "'if' b 'then' c 'else' c'" :=
-  (If b c c')
-  (in custom com at level 10, c at next level, c' at next level) : com_scope.
-
-Definition Assert b := <{ (assume b) ⨁ ((assume ~ b) ; error()) }>.
-
-Notation "'assert' '(' c ')' " :=
-  (Assert c) (in custom com at level 8) : com_scope.
-
-Fixpoint Cpow (C: com) (n: nat): com := 
-match n with
-| 0 => <{skip}>
-| S m => <{ C ; Cpow C m }>
-end.
-
-Infix "^" := Cpow (in custom com at level 10).
-
-(* Notation "c '^' n" :=
-  (Cpow c n) (in custom com at level 8) : com_scope. *)
-
-Reserved Notation
-         "st '=[' c ']=>' ϵ ':' st'"
-         (at level 40, c custom com at level 99,
-          st constr, ϵ constr at next level).
-
-Inductive Signal: Type := 
-| ok
-| err.
-
-Inductive ceval : com -> state -> Signal -> state -> Prop :=
-| E_Skip : forall st eps,
-  st =[ skip ]=> eps : st
-| E_Local : forall st st' x v c ϵ,
-  (x !-> v ; st) =[ local x . c ]=> ϵ : (x !-> v ; st')
-| E_Asgn : forall st a n x,
-  aeval st a = Some n ->
-  st =[ x := a ]=> ok : (x !-> n ; st)
-(* Alternative version
-| E_Asgn : forall st a n x st',
-  aeval st a = n ->
-  st' = (x !-> n ; st) ->
-  st =[ x := a ]=> ok : st' *)
-| E_Seq_Norm : forall c1 c2 st st' st'' ϵ,
-  st =[ c1 ]=> ok : st' ->
-  st' =[ c2 ]=> ϵ : st'' ->
-  st =[ c1 ; c2 ]=> ϵ : st''
-| E_Seq_Err : forall c1 c2 st st',
-  st =[ c1 ]=> err : st' ->
-  st =[ c1 ; c2 ]=> err : st'
- | E_Assume : forall st b,
-  beval st b = true ->
-  st =[ assume b ]=> ok : st
-| E_ErrorOk:
-  empty =[ error() ]=> ok: empty
-| E_Error: forall st,
-  st =[ error() ]=> err: st
-| E_StarSkip : forall c st ϵ,
-  st =[ skip ]=> ϵ : st -> 
-  st =[ c ⋆ ]=> ϵ : st
-| E_StarIter : forall c st st' st'' ϵ,
-  st =[ c ⋆ ]=> ok : st' ->
-  st' =[ c ]=> ϵ : st'' -> 
-  st =[ c ⋆ ]=> ϵ : st''
-| E_StarIter_Err : forall c st,
-  st =[ c ⋆ ]=> err : st
-| E_ChoiceLeft: forall x y st st' ϵ,
-  st =[ x ]=> ϵ : st' ->
-  st =[ x ⨁ y ]=> ϵ : st'
-| E_ChoiceRight: forall x y st st' ϵ,
-  st =[ y ]=> ϵ : st' ->
-  st =[ x ⨁ y ]=> ϵ : st'
-| E_Nondet: forall x st n,
-  st =[ nondet x ]=> ok : (x !-> n ; st)
-where "st =[ c ]=> ϵ : st'" := (ceval c st ϵ st').
-
-Local Hint Constructors ceval : core.
-
-Definition Assertion := state -> Prop.
-
-Definition Aexp : Type := state -> option nat.
-Definition assert_of_Prop (P : Prop) : Assertion := fun _ => P.
-Definition Aexp_of_nat (n : nat) : Aexp := fun _ => Some n.
-Definition Aexp_of_aexp (a : aexp) : Aexp := fun st => aeval st a.
-
-(* Sortclass, the class of sorts; its objects are the terms whose type is a sort (e.g. Prop or Type).  *)
-Coercion assert_of_Prop : Sortclass >-> Assertion.
-Coercion Aexp_of_nat : nat >-> Aexp.
-Coercion Aexp_of_aexp : aexp >-> Aexp.
-
-Arguments assert_of_Prop /.
-Arguments Aexp_of_nat /.
-Arguments Aexp_of_aexp /.
-Add Printing Coercion Aexp_of_nat Aexp_of_aexp assert_of_Prop.
-
-Declare Scope assertion_scope.
-Bind Scope assertion_scope with Assertion.
-Bind Scope assertion_scope with Aexp.
-Delimit Scope assertion_scope with assertion.
-Notation assertion P := (P%assertion : Assertion).
-Notation mkAexp a := (a%assertion : Aexp).
-Notation "~ P" := (fun st => ~ assertion P st) : assertion_scope.
-Notation "P /\ Q" := (fun st => assertion P st /\  assertion Q st) : assertion_scope.
-Notation "P \/ Q" := (fun st => assertion P st \/ assertion Q st) : assertion_scope.
-Notation "P -> Q" := (fun st => assertion P st -> assertion Q st) : assertion_scope.
-Notation "P <-> Q" := (fun st => assertion P st <-> assertion Q st) : assertion_scope.
-Notation "a = b" := (fun st => mkAexp a st = mkAexp b st) : assertion_scope.
-Notation "a + b" := (fun st => mkAexp a st + mkAexp b st) : assertion_scope.
-
-Definition assert_implies (P Q : Assertion) : Prop :=
-  forall st, P st -> Q st.
-
-Declare Scope inclogic_spec_scope.
-
-Notation "P ->> Q" := (assert_implies P Q)
-                      (at level 80) : inclogic_spec_scope.
-Open Scope inclogic_spec_scope.
-
-Notation "P <<->> Q" :=
-  (P ->> Q /\ Q ->> P) (at level 80) : inclogic_spec_scope.
-
-
-(* P' that is just like P except that, wherever P looks up the variable X in the current state, P' instead uses the value of the expression a. *)
-Definition assn_sub X a P : Assertion :=
-  fun (st : state) =>
-    exists v, (aeval st a) = Some v -> P (set st X v).
-
-Notation "P [ X |-> a ]" := (assn_sub X a P) (at level 10).
-
-Hint Unfold assert_implies : core.
-
-
-(* substAexp x y a, which replaces all occurrences of a variable x with a value y inside an arithmetic expression a. *)
-Fixpoint substAexp (x: string) (y: aexp) (a: aexp) : aexp :=
-match a with
-  | ANum n => ANum n
-  | AId var => if String.eqb x var then y else (AId var)
-  | <{a1 + a2}> => <{(substAexp x y a1) + (substAexp x y a2)}>
-  | <{a1 - a2}> => <{(substAexp x y a1) - (substAexp x y a2)}>
-  | <{a1 * a2}> => <{(substAexp x y a1) * (substAexp x y a2)}>
-end.
-
-(* substBeval x y b, which replaces all occurrences of a variable x with a value y inside a boolean expression b. *)
-Fixpoint substBeval (x: string) (y: aexp) (b: bexp) : bexp :=
-let auxa t := substAexp x y t in
-let aux t := substBeval x y t in
-match b with
-| BTrue => BTrue
-| BFalse => BFalse
-| BEq a1 a2 => BEq (auxa a1) (auxa a2)
-| BNot b => aux b
-| <{ a1 <= a2 }> => <{ auxa a1 <= auxa a2 }>
-| <{ b1 //\\ b2 }> => <{(aux b1) //\\ (aux b2)}>
-end.
-
-(* subst x y c, which replaces all occurrences of a variable x with a value y inside a command c. *)
-Fixpoint substCmd (x: string) (y: aexp) (c: com) : com :=
-let aux t := substCmd x y t in
-match y with 
-| AId yvar => 
-  let if_y_eq z t1 t2 := if String.eqb x z then t1 (* update *) else t2 (* skip *) in
-  match c with
-  | Skip => Skip
-  | Asign x' v =>  if_y_eq x' (Asign yvar (substAexp x y v)) (Asign x' (substAexp x y v)) 
-  | Seq c1 c2 => Seq (aux c1) (aux c2) 
-  | Assume b => Assume b
-  | Error => Error
-  | Star c => Star (aux c)
-  | Choice c1 c2 => Choice (aux c1) (aux c2)
-  | CLocal x' c' => if_y_eq x' (CLocal yvar (aux c')) (CLocal x' (aux c'))
-  | Nondet x' => if_y_eq x' (Nondet yvar) (Nondet x')
-  end
-| w => 
-  match c with
-  | Skip => Skip
-  | Asign var exp =>  (Asign var (substAexp x w exp))
-  | Seq c1 c2 => Seq (aux c1) (aux c2) 
-  | Assume b => Assume (substBeval x w b)
-  | Error => Error
-  | Star c => Star (aux c)
-  | Choice c1 c2 => Choice (aux c1) (aux c2)
-  | CLocal x' c' => (CLocal x' (aux c'))
-  | Nondet x' => Nondet x'
-  end
-end.
-
-Example testsubstCmd: substCmd "X"%string (AId "Y"%string)
-  <{ "X" := (AId "X"%string); skip; "Z" :=  (AId "X"%string)}> 
-  = <{ "Y" := (AId "Y"%string); skip; "Z" :=  (AId "Y"%string)}>.
-Proof. reflexivity. Qed.
-
-Example testsubstCmd2: substCmd "X"%string (APlus (ANum 1) (ANum 1))
-  <{ "Y" := (AId "X"%string); skip; "Z" :=  (APlus (ANum 1) (AId "X"%string))}> 
-  = <{ "Y" := (APlus (ANum 1) (ANum 1)); skip; "Z" := (APlus (ANum 1) (APlus (ANum 1) (ANum 1)))}>.
-Proof. reflexivity. Qed.
-
-
-(* - apply (E_Seq_Norm c <{ c ⋆ }> _ _ _ _ H6 H2). *)
-
-(* induction c; inversion H; subst.
-- econstructor. apply H6. *)
-
-
-Hint Unfold assert_implies : core.
-Hint Unfold assert_of_Prop Aexp_of_nat Aexp_of_aexp : core.
+Corollary reds_to_cexec_error:
+  forall s c s',
+    star red (c, s) (ERROR, s') -> s =[ c ]=> RError.
+Proof.
+  intros s c s' STAR.
+  apply reds_to_cexec.
+  exists (ERROR, s'). split; [exact STAR | constructor].
+Qed.
